I can now compile Dan Ellison's echo smart contract.

elle/generated/FourL.ml
@@ -1,0 +1,1385 @@
+module FourL : sig
+  val compiler : string -> string option
+end = struct
+
+type int = Int_of_integer of Big_int.big_int;;
+
+type num = One | Bit0 of num | Bit1 of num;;
+
+let one_inta : int = Int_of_integer (Big_int.big_int_of_int 1);;
+
+type 'a one = {one : 'a};;
+let one _A = _A.one;;
+
+let one_int = ({one = one_inta} : int one);;
+
+let rec integer_of_int (Int_of_integer k) = k;;
+
+let rec times_inta
+  k l = Int_of_integer
+          (Big_int.mult_big_int (integer_of_int k) (integer_of_int l));;
+
+type 'a times = {times : 'a -> 'a -> 'a};;
+let times _A = _A.times;;
+
+type 'a power = {one_power : 'a one; times_power : 'a times};;
+
+let times_int = ({times = times_inta} : int times);;
+
+let power_int = ({one_power = one_int; times_power = times_int} : int power);;
+
+type 'a equal = {equal : 'a -> 'a -> bool};;
+let equal _A = _A.equal;;
+
+let equal_char = ({equal = (fun a b -> ((a : char) = b))} : char equal);;
+
+type nat = Nat of Big_int.big_int;;
+
+type 'a itself = Type;;
+
+type 'a len0 = {len_of : 'a itself -> nat};;
+let len_of _A = _A.len_of;;
+
+let rec integer_of_nat (Nat x) = x;;
+
+let rec times_nat
+  m n = Nat (Big_int.mult_big_int (integer_of_nat m) (integer_of_nat n));;
+
+type 'a ord = {less_eq : 'a -> 'a -> bool; less : 'a -> 'a -> bool};;
+let less_eq _A = _A.less_eq;;
+let less _A = _A.less;;
+
+let rec max _A a b = (if less_eq _A a b then b else a);;
+
+let ord_integer =
+  ({less_eq = Big_int.le_big_int; less = Big_int.lt_big_int} :
+    Big_int.big_int ord);;
+
+let rec nat_of_integer k = Nat (max ord_integer Big_int.zero_big_int k);;
+
+type 'a finite = unit;;
+
+type 'a bit0 = Abs_bit0 of int;;
+
+let rec len_of_bit0 _A
+  uu = times_nat (nat_of_integer (Big_int.big_int_of_int 2)) (len_of _A Type);;
+
+let rec len0_bit0 _A = ({len_of = len_of_bit0 _A} : 'a bit0 len0);;
+
+let one_nat : nat = Nat (Big_int.big_int_of_int 1);;
+
+type num1 = One_num1;;
+
+let rec len_of_num1 uu = one_nat;;
+
+let len0_num1 = ({len_of = len_of_num1} : num1 len0);;
+
+type storage_inst = SLOAD | SSTORE;;
+
+type sarith_inst = SDIV | SMOD | SGT | SLT | SIGNEXTEND;;
+
+type memory_inst = MLOAD | MSTORE | MSTORE8 | CALLDATACOPY | CODECOPY |
+  EXTCODECOPY | MSIZE;;
+
+type 'a word = Word of int;;
+
+type stack_inst = POP | PUSH_N of num1 bit0 bit0 bit0 word list | CALLDATALOAD;;
+
+type arith_inst = ADD | MUL | SUB | DIV | MOD | ADDMOD | MULMOD | EXP | Inst_GT
+  | Inst_EQ | Inst_LT | ISZERO | SHA3;;
+
+type misc_inst = STOP | CREATE | CALL | CALLCODE | DELEGATECALL | RETURN |
+  SUICIDE;;
+
+type info_inst = ADDRESS | BALANCE | ORIGIN | CALLER | CALLVALUE | CALLDATASIZE
+  | CODESIZE | GASPRICE | EXTCODESIZE | BLOCKHASH | COINBASE | TIMESTAMP |
+  NUMBER | DIFFICULTY | GASLIMIT | GAS;;
+
+type bits_inst = Inst_AND | Inst_OR | Inst_XOR | Inst_NOT | BYTE;;
+
+type log_inst = LOG0 | LOG1 | LOG2 | LOG3 | LOG4;;
+
+type pc_inst = JUMP | JUMPI | PC | JUMPDEST;;
+
+type inst = Unknown of num1 bit0 bit0 bit0 word | Bits of bits_inst |
+  Sarith of sarith_inst | Arith of arith_inst | Info of info_inst |
+  Dup of num1 bit0 bit0 word | Memory of memory_inst | Storage of storage_inst |
+  Pc of pc_inst | Stack of stack_inst | Swap of num1 bit0 bit0 word |
+  Log of log_inst | Misc of misc_inst;;
+
+type llllcompare = LCEq | LCNeq | LCLt | LCLe | LCGt | LCGe;;
+
+type lllllogic = LLAnd | LLOr | LLNot;;
+
+type llllarith = LAPlus | LAMinus | LATimes | LADiv | LAMod | LAAnd | LAOr |
+  LAXor | LANot | LAExp;;
+
+type llll = L4L_Str of char list | L4L_Nat of nat | L4I0 of inst |
+  L4I1 of inst * llll | L4I2 of inst * llll * llll | L4Seq of llll list |
+  L4Arith of llllarith * llll list | L4Logic of lllllogic * llll list |
+  L4Comp of llllcompare * llll * llll | L4When of llll * llll |
+  L4If of llll * llll * llll | L4While of llll * llll;;
+
+type stree = STStr of char list | STStrs of stree list;;
+
+type ll1 = L of inst | LLab of nat | LJmp of nat | LJmpI of nat |
+  LSeq of ll1 list;;
+
+type ('a, 'b, 'c, 'd, 'e, 'f, 'g) llt = La of 'a * inst | LLaba of 'b * nat |
+  LJmpa of 'c * nat * nat | LJmpIa of 'd * nat * nat |
+  LSeqa of 'e * ((nat * nat) * ('a, 'b, 'c, 'd, 'e, 'f, 'g) llt) list;;
+
+type jump_resolve_result = JSuccess | JFail of nat list | JBump of nat list;;
+
+let rec eq _A a b = equal _A a b;;
+
+let rec nat k = Nat (max ord_integer Big_int.zero_big_int (integer_of_int k));;
+
+let rec plus_nat
+  m n = Nat (Big_int.add_big_int (integer_of_nat m) (integer_of_nat n));;
+
+let rec suc n = plus_nat n one_nat;;
+
+let rec comp f g = (fun x -> f (g x));;
+
+let rec fold f x1 s = match f, x1, s with f, x :: xs, s -> fold f xs (f x s)
+               | f, [], s -> s;;
+
+let rec rev xs = fold (fun a b -> a :: b) xs [];;
+
+let rec maps f x1 = match f, x1 with f, [] -> []
+               | f, x :: xs -> f x @ maps f xs;;
+
+let rec null = function [] -> true
+               | x :: xs -> false;;
+
+let rec uint _A (Word x) = x;;
+
+let rec unat _A w = nat (uint _A w);;
+
+let rec char_of_nat
+  x = comp (fun a -> Char.chr (Big_int.int_of_big_int a)) integer_of_nat x;;
+
+let apos : char = char_of_nat (nat_of_integer (Big_int.big_int_of_int 39));;
+
+let zero_nat : nat = Nat Big_int.zero_big_int;;
+
+let rec gen_length n x1 = match n, x1 with n, x :: xs -> gen_length (suc n) xs
+                     | n, [] -> n;;
+
+let rec size_list x = gen_length zero_nat x;;
+
+let rec int_of_nat n = Int_of_integer (integer_of_nat n);;
+
+let rec sgn_integer
+  k = (if Big_int.eq_big_int k Big_int.zero_big_int then Big_int.zero_big_int
+        else (if Big_int.lt_big_int k Big_int.zero_big_int
+               then (Big_int.minus_big_int (Big_int.big_int_of_int 1))
+               else (Big_int.big_int_of_int 1)));;
+
+let rec apsnd f (x, y) = (x, f y);;
+
+let rec divmod_integer
+  k l = (if Big_int.eq_big_int k Big_int.zero_big_int
+          then (Big_int.zero_big_int, Big_int.zero_big_int)
+          else (if Big_int.eq_big_int l Big_int.zero_big_int
+                 then (Big_int.zero_big_int, k)
+                 else comp (comp apsnd Big_int.mult_big_int) sgn_integer l
+                        (if Big_int.eq_big_int (sgn_integer k) (sgn_integer l)
+                          then Big_int.quomod_big_int (Big_int.abs_big_int k)
+                                 (Big_int.abs_big_int l)
+                          else (let (r, s) =
+                                  Big_int.quomod_big_int (Big_int.abs_big_int k)
+                                    (Big_int.abs_big_int l)
+                                  in
+                                 (if Big_int.eq_big_int s Big_int.zero_big_int
+                                   then (Big_int.minus_big_int r,
+  Big_int.zero_big_int)
+                                   else (Big_int.sub_big_int
+   (Big_int.minus_big_int r) (Big_int.big_int_of_int 1),
+  Big_int.sub_big_int (Big_int.abs_big_int l) s))))));;
+
+let rec snd (x1, x2) = x2;;
+
+let rec modulo_integer k l = snd (divmod_integer k l);;
+
+let rec modulo_int
+  k l = Int_of_integer (modulo_integer (integer_of_int k) (integer_of_int l));;
+
+let rec minus_nat
+  m n = Nat (max ord_integer Big_int.zero_big_int
+              (Big_int.sub_big_int (integer_of_nat m) (integer_of_nat n)));;
+
+let rec equal_nat
+  m n = Big_int.eq_big_int (integer_of_nat m) (integer_of_nat n);;
+
+let rec power _A
+  a n = (if equal_nat n zero_nat then one _A.one_power
+          else times _A.times_power a (power _A a (minus_nat n one_nat)));;
+
+let rec word_of_int _A
+  k = Word (modulo_int k
+             (power power_int (Int_of_integer (Big_int.big_int_of_int 2))
+               (len_of _A Type)));;
+
+let rec storage_inst_code
+  = function
+    SLOAD ->
+      word_of_int (len0_bit0 (len0_bit0 (len0_bit0 len0_num1)))
+        (Int_of_integer (Big_int.big_int_of_int 84))
+    | SSTORE ->
+        word_of_int (len0_bit0 (len0_bit0 (len0_bit0 len0_num1)))
+          (Int_of_integer (Big_int.big_int_of_int 85));;
+
+let rec sarith_inst_code
+  = function
+    SDIV ->
+      word_of_int (len0_bit0 (len0_bit0 (len0_bit0 len0_num1)))
+        (Int_of_integer (Big_int.big_int_of_int 5))
+    | SMOD ->
+        word_of_int (len0_bit0 (len0_bit0 (len0_bit0 len0_num1)))
+          (Int_of_integer (Big_int.big_int_of_int 7))
+    | SGT ->
+        word_of_int (len0_bit0 (len0_bit0 (len0_bit0 len0_num1)))
+          (Int_of_integer (Big_int.big_int_of_int 19))
+    | SLT ->
+        word_of_int (len0_bit0 (len0_bit0 (len0_bit0 len0_num1)))
+          (Int_of_integer (Big_int.big_int_of_int 18))
+    | SIGNEXTEND ->
+        word_of_int (len0_bit0 (len0_bit0 (len0_bit0 len0_num1)))
+          (Int_of_integer (Big_int.big_int_of_int 11));;
+
+let rec memory_inst_code
+  = function
+    MLOAD ->
+      word_of_int (len0_bit0 (len0_bit0 (len0_bit0 len0_num1)))
+        (Int_of_integer (Big_int.big_int_of_int 81))
+    | MSTORE ->
+        word_of_int (len0_bit0 (len0_bit0 (len0_bit0 len0_num1)))
+          (Int_of_integer (Big_int.big_int_of_int 82))
+    | MSTORE8 ->
+        word_of_int (len0_bit0 (len0_bit0 (len0_bit0 len0_num1)))
+          (Int_of_integer (Big_int.big_int_of_int 83))
+    | CALLDATACOPY ->
+        word_of_int (len0_bit0 (len0_bit0 (len0_bit0 len0_num1)))
+          (Int_of_integer (Big_int.big_int_of_int 55))
+    | CODECOPY ->
+        word_of_int (len0_bit0 (len0_bit0 (len0_bit0 len0_num1)))
+          (Int_of_integer (Big_int.big_int_of_int 57))
+    | EXTCODECOPY ->
+        word_of_int (len0_bit0 (len0_bit0 (len0_bit0 len0_num1)))
+          (Int_of_integer (Big_int.big_int_of_int 60))
+    | MSIZE ->
+        word_of_int (len0_bit0 (len0_bit0 (len0_bit0 len0_num1)))
+          (Int_of_integer (Big_int.big_int_of_int 89));;
+
+let rec plus_int
+  k l = Int_of_integer
+          (Big_int.add_big_int (integer_of_int k) (integer_of_int l));;
+
+let rec plus_word _A a b = word_of_int _A (plus_int (uint _A a) (uint _A b));;
+
+let zero_int : int = Int_of_integer Big_int.zero_big_int;;
+
+let rec less_nat
+  m n = Big_int.lt_big_int (integer_of_nat m) (integer_of_nat n);;
+
+let rec word8FromNat
+  i = word_of_int (len0_bit0 (len0_bit0 (len0_bit0 len0_num1))) (int_of_nat i);;
+
+let rec byteFromNat x = word8FromNat x;;
+
+let rec stack_inst_code
+  = function
+    POP ->
+      [word_of_int (len0_bit0 (len0_bit0 (len0_bit0 len0_num1)))
+         (Int_of_integer (Big_int.big_int_of_int 80))]
+    | PUSH_N lst ->
+        (if less_nat (size_list lst) one_nat
+          then [word_of_int (len0_bit0 (len0_bit0 (len0_bit0 len0_num1)))
+                  (Int_of_integer (Big_int.big_int_of_int 96));
+                 word_of_int (len0_bit0 (len0_bit0 (len0_bit0 len0_num1)))
+                   zero_int]
+          else (if less_nat (nat_of_integer (Big_int.big_int_of_int 32))
+                     (size_list lst)
+                 then [word_of_int (len0_bit0 (len0_bit0 (len0_bit0 len0_num1)))
+                         (Int_of_integer (Big_int.big_int_of_int 96));
+                        word_of_int
+                          (len0_bit0 (len0_bit0 (len0_bit0 len0_num1)))
+                          zero_int]
+                 else [plus_word (len0_bit0 (len0_bit0 (len0_bit0 len0_num1)))
+                         (byteFromNat (size_list lst))
+                         (word_of_int
+                           (len0_bit0 (len0_bit0 (len0_bit0 len0_num1)))
+                           (Int_of_integer (Big_int.big_int_of_int 95)))] @
+                        lst))
+    | CALLDATALOAD ->
+        [word_of_int (len0_bit0 (len0_bit0 (len0_bit0 len0_num1)))
+           (Int_of_integer (Big_int.big_int_of_int 53))];;
+
+let rec arith_inst_code
+  = function
+    ADD -> word_of_int (len0_bit0 (len0_bit0 (len0_bit0 len0_num1))) one_inta
+    | MUL ->
+        word_of_int (len0_bit0 (len0_bit0 (len0_bit0 len0_num1)))
+          (Int_of_integer (Big_int.big_int_of_int 2))
+    | SUB ->
+        word_of_int (len0_bit0 (len0_bit0 (len0_bit0 len0_num1)))
+          (Int_of_integer (Big_int.big_int_of_int 3))
+    | DIV ->
+        word_of_int (len0_bit0 (len0_bit0 (len0_bit0 len0_num1)))
+          (Int_of_integer (Big_int.big_int_of_int 4))
+    | MOD ->
+        word_of_int (len0_bit0 (len0_bit0 (len0_bit0 len0_num1)))
+          (Int_of_integer (Big_int.big_int_of_int 6))
+    | ADDMOD ->
+        word_of_int (len0_bit0 (len0_bit0 (len0_bit0 len0_num1)))
+          (Int_of_integer (Big_int.big_int_of_int 8))
+    | MULMOD ->
+        word_of_int (len0_bit0 (len0_bit0 (len0_bit0 len0_num1)))
+          (Int_of_integer (Big_int.big_int_of_int 9))
+    | EXP ->
+        word_of_int (len0_bit0 (len0_bit0 (len0_bit0 len0_num1)))
+          (Int_of_integer (Big_int.big_int_of_int 10))
+    | Inst_GT ->
+        word_of_int (len0_bit0 (len0_bit0 (len0_bit0 len0_num1)))
+          (Int_of_integer (Big_int.big_int_of_int 17))
+    | Inst_LT ->
+        word_of_int (len0_bit0 (len0_bit0 (len0_bit0 len0_num1)))
+          (Int_of_integer (Big_int.big_int_of_int 16))
+    | Inst_EQ ->
+        word_of_int (len0_bit0 (len0_bit0 (len0_bit0 len0_num1)))
+          (Int_of_integer (Big_int.big_int_of_int 20))
+    | ISZERO ->
+        word_of_int (len0_bit0 (len0_bit0 (len0_bit0 len0_num1)))
+          (Int_of_integer (Big_int.big_int_of_int 21))
+    | SHA3 ->
+        word_of_int (len0_bit0 (len0_bit0 (len0_bit0 len0_num1)))
+          (Int_of_integer (Big_int.big_int_of_int 32));;
+
+let rec swap_inst_code
+  m = plus_word (len0_bit0 (len0_bit0 (len0_bit0 len0_num1)))
+        (word_of_int (len0_bit0 (len0_bit0 (len0_bit0 len0_num1)))
+          (uint (len0_bit0 (len0_bit0 len0_num1)) m))
+        (word_of_int (len0_bit0 (len0_bit0 (len0_bit0 len0_num1)))
+          (Int_of_integer (Big_int.big_int_of_int 144)));;
+
+let rec misc_inst_code
+  = function
+    STOP -> word_of_int (len0_bit0 (len0_bit0 (len0_bit0 len0_num1))) zero_int
+    | CREATE ->
+        word_of_int (len0_bit0 (len0_bit0 (len0_bit0 len0_num1)))
+          (Int_of_integer (Big_int.big_int_of_int 240))
+    | CALL ->
+        word_of_int (len0_bit0 (len0_bit0 (len0_bit0 len0_num1)))
+          (Int_of_integer (Big_int.big_int_of_int 241))
+    | CALLCODE ->
+        word_of_int (len0_bit0 (len0_bit0 (len0_bit0 len0_num1)))
+          (Int_of_integer (Big_int.big_int_of_int 242))
+    | RETURN ->
+        word_of_int (len0_bit0 (len0_bit0 (len0_bit0 len0_num1)))
+          (Int_of_integer (Big_int.big_int_of_int 243))
+    | DELEGATECALL ->
+        word_of_int (len0_bit0 (len0_bit0 (len0_bit0 len0_num1)))
+          (Int_of_integer (Big_int.big_int_of_int 244))
+    | SUICIDE ->
+        word_of_int (len0_bit0 (len0_bit0 (len0_bit0 len0_num1)))
+          (Int_of_integer (Big_int.big_int_of_int 255));;
+
+let rec info_inst_code
+  = function
+    ADDRESS ->
+      word_of_int (len0_bit0 (len0_bit0 (len0_bit0 len0_num1)))
+        (Int_of_integer (Big_int.big_int_of_int 48))
+    | BALANCE ->
+        word_of_int (len0_bit0 (len0_bit0 (len0_bit0 len0_num1)))
+          (Int_of_integer (Big_int.big_int_of_int 49))
+    | ORIGIN ->
+        word_of_int (len0_bit0 (len0_bit0 (len0_bit0 len0_num1)))
+          (Int_of_integer (Big_int.big_int_of_int 50))
+    | CALLVALUE ->
+        word_of_int (len0_bit0 (len0_bit0 (len0_bit0 len0_num1)))
+          (Int_of_integer (Big_int.big_int_of_int 52))
+    | CALLDATASIZE ->
+        word_of_int (len0_bit0 (len0_bit0 (len0_bit0 len0_num1)))
+          (Int_of_integer (Big_int.big_int_of_int 54))
+    | CALLER ->
+        word_of_int (len0_bit0 (len0_bit0 (len0_bit0 len0_num1)))
+          (Int_of_integer (Big_int.big_int_of_int 51))
+    | CODESIZE ->
+        word_of_int (len0_bit0 (len0_bit0 (len0_bit0 len0_num1)))
+          (Int_of_integer (Big_int.big_int_of_int 56))
+    | GASPRICE ->
+        word_of_int (len0_bit0 (len0_bit0 (len0_bit0 len0_num1)))
+          (Int_of_integer (Big_int.big_int_of_int 58))
+    | EXTCODESIZE ->
+        word_of_int (len0_bit0 (len0_bit0 (len0_bit0 len0_num1)))
+          (Int_of_integer (Big_int.big_int_of_int 59))
+    | BLOCKHASH ->
+        word_of_int (len0_bit0 (len0_bit0 (len0_bit0 len0_num1)))
+          (Int_of_integer (Big_int.big_int_of_int 64))
+    | COINBASE ->
+        word_of_int (len0_bit0 (len0_bit0 (len0_bit0 len0_num1)))
+          (Int_of_integer (Big_int.big_int_of_int 65))
+    | TIMESTAMP ->
+        word_of_int (len0_bit0 (len0_bit0 (len0_bit0 len0_num1)))
+          (Int_of_integer (Big_int.big_int_of_int 66))
+    | NUMBER ->
+        word_of_int (len0_bit0 (len0_bit0 (len0_bit0 len0_num1)))
+          (Int_of_integer (Big_int.big_int_of_int 67))
+    | DIFFICULTY ->
+        word_of_int (len0_bit0 (len0_bit0 (len0_bit0 len0_num1)))
+          (Int_of_integer (Big_int.big_int_of_int 68))
+    | GASLIMIT ->
+        word_of_int (len0_bit0 (len0_bit0 (len0_bit0 len0_num1)))
+          (Int_of_integer (Big_int.big_int_of_int 69))
+    | GAS ->
+        word_of_int (len0_bit0 (len0_bit0 (len0_bit0 len0_num1)))
+          (Int_of_integer (Big_int.big_int_of_int 90));;
+
+let rec bits_inst_code
+  = function
+    Inst_AND ->
+      word_of_int (len0_bit0 (len0_bit0 (len0_bit0 len0_num1)))
+        (Int_of_integer (Big_int.big_int_of_int 22))
+    | Inst_OR ->
+        word_of_int (len0_bit0 (len0_bit0 (len0_bit0 len0_num1)))
+          (Int_of_integer (Big_int.big_int_of_int 23))
+    | Inst_XOR ->
+        word_of_int (len0_bit0 (len0_bit0 (len0_bit0 len0_num1)))
+          (Int_of_integer (Big_int.big_int_of_int 24))
+    | Inst_NOT ->
+        word_of_int (len0_bit0 (len0_bit0 (len0_bit0 len0_num1)))
+          (Int_of_integer (Big_int.big_int_of_int 25))
+    | BYTE ->
+        word_of_int (len0_bit0 (len0_bit0 (len0_bit0 len0_num1)))
+          (Int_of_integer (Big_int.big_int_of_int 26));;
+
+let rec log_inst_code
+  = function
+    LOG0 ->
+      word_of_int (len0_bit0 (len0_bit0 (len0_bit0 len0_num1)))
+        (Int_of_integer (Big_int.big_int_of_int 160))
+    | LOG1 ->
+        word_of_int (len0_bit0 (len0_bit0 (len0_bit0 len0_num1)))
+          (Int_of_integer (Big_int.big_int_of_int 161))
+    | LOG2 ->
+        word_of_int (len0_bit0 (len0_bit0 (len0_bit0 len0_num1)))
+          (Int_of_integer (Big_int.big_int_of_int 162))
+    | LOG3 ->
+        word_of_int (len0_bit0 (len0_bit0 (len0_bit0 len0_num1)))
+          (Int_of_integer (Big_int.big_int_of_int 163))
+    | LOG4 ->
+        word_of_int (len0_bit0 (len0_bit0 (len0_bit0 len0_num1)))
+          (Int_of_integer (Big_int.big_int_of_int 164));;
+
+let rec dup_inst_code
+  m = plus_word (len0_bit0 (len0_bit0 (len0_bit0 len0_num1)))
+        (word_of_int (len0_bit0 (len0_bit0 (len0_bit0 len0_num1)))
+          (uint (len0_bit0 (len0_bit0 len0_num1)) m))
+        (word_of_int (len0_bit0 (len0_bit0 (len0_bit0 len0_num1)))
+          (Int_of_integer (Big_int.big_int_of_int 128)));;
+
+let rec pc_inst_code
+  = function
+    JUMP ->
+      word_of_int (len0_bit0 (len0_bit0 (len0_bit0 len0_num1)))
+        (Int_of_integer (Big_int.big_int_of_int 86))
+    | JUMPI ->
+        word_of_int (len0_bit0 (len0_bit0 (len0_bit0 len0_num1)))
+          (Int_of_integer (Big_int.big_int_of_int 87))
+    | PC -> word_of_int (len0_bit0 (len0_bit0 (len0_bit0 len0_num1)))
+              (Int_of_integer (Big_int.big_int_of_int 88))
+    | JUMPDEST ->
+        word_of_int (len0_bit0 (len0_bit0 (len0_bit0 len0_num1)))
+          (Int_of_integer (Big_int.big_int_of_int 91));;
+
+let rec inst_code = function Unknown byte -> [byte]
+                    | Bits b -> [bits_inst_code b]
+                    | Sarith s -> [sarith_inst_code s]
+                    | Arith a -> [arith_inst_code a]
+                    | Info i -> [info_inst_code i]
+                    | Dup d -> [dup_inst_code d]
+                    | Memory m -> [memory_inst_code m]
+                    | Storage s -> [storage_inst_code s]
+                    | Pc p -> [pc_inst_code p]
+                    | Stack s -> stack_inst_code s
+                    | Swap s -> [swap_inst_code s]
+                    | Log l -> [log_inst_code l]
+                    | Misc m -> [misc_inst_code m];;
+
+let rec inst_size i = int_of_nat (size_list (inst_code i));;
+
+let rec ilsz = function [] -> zero_nat
+               | h :: t -> plus_nat (nat (inst_size h)) (ilsz t);;
+
+let rec map f x1 = match f, x1 with f, [] -> []
+              | f, x21 :: x22 -> f x21 :: map f x22;;
+
+let rec member _A x0 y = match x0, y with [], y -> false
+                    | x :: xs, y -> eq _A x y || member _A xs y;;
+
+let rec isWs
+  x = member equal_char
+        (map char_of_nat
+          [nat_of_integer (Big_int.big_int_of_int 9);
+            nat_of_integer (Big_int.big_int_of_int 10);
+            nat_of_integer (Big_int.big_int_of_int 11);
+            nat_of_integer (Big_int.big_int_of_int 12);
+            nat_of_integer (Big_int.big_int_of_int 13);
+            nat_of_integer (Big_int.big_int_of_int 32)])
+        x;;
+
+let rec foldl f a x2 = match f, a, x2 with f, a, [] -> a
+                | f, a, x :: xs -> foldl f (f a x) xs;;
+
+let rec map_of _A
+  x0 k = match x0, k with
+    (l, v) :: ps, k -> (if eq _A l k then Some v else map_of _A ps k)
+    | [], k -> None;;
+
+let rec il2wl il = maps inst_code il;;
+
+let rec equal_list _A
+  x0 x1 = match x0, x1 with [], x21 :: x22 -> false
+    | x21 :: x22, [] -> false
+    | x21 :: x22, y21 :: y22 -> eq _A x21 y21 && equal_list _A x22 y22
+    | [], [] -> true;;
+
+let rec lookupS
+  x0 uu = match x0, uu with [], uu -> None
+    | (ah, bh) :: t, a ->
+        (if equal_list equal_char a ah then Some bh else lookupS t a);;
+
+let rec mkConsts
+  x0 x1 = match x0, x1 with [], [] -> Some []
+    | sh :: st, lh :: lt ->
+        (match mkConsts st lt with None -> None
+          | Some ft -> Some ((sh, (fun _ -> Some lh)) :: ft))
+    | v :: va, [] -> None
+    | [], v :: va -> None;;
+
+let hex_parse_table : (char * nat) list
+  = [('0', zero_nat); ('1', one_nat);
+      ('2', nat_of_integer (Big_int.big_int_of_int 2));
+      ('3', nat_of_integer (Big_int.big_int_of_int 3));
+      ('4', nat_of_integer (Big_int.big_int_of_int 4));
+      ('5', nat_of_integer (Big_int.big_int_of_int 5));
+      ('6', nat_of_integer (Big_int.big_int_of_int 6));
+      ('7', nat_of_integer (Big_int.big_int_of_int 7));
+      ('8', nat_of_integer (Big_int.big_int_of_int 8));
+      ('9', nat_of_integer (Big_int.big_int_of_int 9));
+      ('A', nat_of_integer (Big_int.big_int_of_int 10));
+      ('a', nat_of_integer (Big_int.big_int_of_int 10));
+      ('B', nat_of_integer (Big_int.big_int_of_int 11));
+      ('b', nat_of_integer (Big_int.big_int_of_int 11));
+      ('C', nat_of_integer (Big_int.big_int_of_int 12));
+      ('c', nat_of_integer (Big_int.big_int_of_int 12));
+      ('D', nat_of_integer (Big_int.big_int_of_int 13));
+      ('d', nat_of_integer (Big_int.big_int_of_int 13));
+      ('E', nat_of_integer (Big_int.big_int_of_int 14));
+      ('e', nat_of_integer (Big_int.big_int_of_int 14));
+      ('F', nat_of_integer (Big_int.big_int_of_int 15));
+      ('f', nat_of_integer (Big_int.big_int_of_int 15))];;
+
+let rec parseHexNumeral
+  x0 s f r = match x0, s, f, r with [], s, f, r -> f []
+    | h :: t, s, f, r ->
+        (match map_of equal_char hex_parse_table h with None -> f (h :: t)
+          | Some n -> s n t);;
+
+let rec parseHexSub
+  i x1 su fa r = match i, x1, su, fa, r with i, [], su, fa, r -> su i []
+    | i, h :: t, su, fa, r ->
+        parseHexNumeral (h :: t)
+          (fun n l ->
+            parseHexSub
+              (plus_nat
+                (times_nat (nat_of_integer (Big_int.big_int_of_int 16)) i) n)
+              l su fa r)
+          (su i) r;;
+
+let rec parseHex
+  x0 su fa r = match x0, su, fa, r with
+    h0 :: hx :: h :: t, su, fa, r ->
+      (if ((h0 : char) = '0') && ((hx : char) = 'x')
+        then parseHexNumeral (h :: t) (fun n l -> parseHexSub n l su fa r) fa r
+        else fa (h0 :: hx :: h :: t))
+    | [], su, fa, r -> fa []
+    | [v], su, fa, r -> fa [v]
+    | [v; vb], su, fa, r -> fa [v; vb];;
+
+let rec is_digit_char
+  c = ((c : char) = '0') ||
+        (((c : char) = '5') ||
+          (((c : char) = '1') ||
+            (((c : char) = '6') ||
+              (((c : char) = '2') ||
+                (((c : char) = '7') ||
+                  (((c : char) = '3') ||
+                    (((c : char) = '8') ||
+                      (((c : char) = '4') || ((c : char) = '9')))))))));;
+
+let rec char_to_digit
+  c = (if ((c : char) = '0') then zero_nat
+        else (if ((c : char) = '1') then one_nat
+               else (if ((c : char) = '2')
+                      then nat_of_integer (Big_int.big_int_of_int 2)
+                      else (if ((c : char) = '3')
+                             then nat_of_integer (Big_int.big_int_of_int 3)
+                             else (if ((c : char) = '4')
+                                    then nat_of_integer
+   (Big_int.big_int_of_int 4)
+                                    else (if ((c : char) = '5')
+   then nat_of_integer (Big_int.big_int_of_int 5)
+   else (if ((c : char) = '6') then nat_of_integer (Big_int.big_int_of_int 6)
+          else (if ((c : char) = '7')
+                 then nat_of_integer (Big_int.big_int_of_int 7)
+                 else (if ((c : char) = '8')
+                        then nat_of_integer (Big_int.big_int_of_int 8)
+                        else (if ((c : char) = '9')
+                               then nat_of_integer (Big_int.big_int_of_int 9)
+                               else nat_of_integer
+                                      (Big_int.big_int_of_int 10)))))))))));;
+
+let rec parseNumeral
+  x0 s f r = match x0, s, f, r with [], s, f, r -> f []
+    | h :: t, s, f, r ->
+        (if is_digit_char h then s (char_to_digit h) t else f (h :: t));;
+
+let rec parseNatSub
+  i x1 su fa r = match i, x1, su, fa, r with i, [], su, fa, r -> su i []
+    | i, h :: t, su, fa, r ->
+        parseNumeral (h :: t)
+          (fun n l ->
+            parseNatSub
+              (plus_nat
+                (times_nat (nat_of_integer (Big_int.big_int_of_int 10)) i) n)
+              l su fa r)
+          (su i) r;;
+
+let rec parseNat
+  x0 su fa r = match x0, su, fa, r with [], su, fa, r -> fa []
+    | h :: t, su, fa, r ->
+        parseNumeral (h :: t) (fun n l -> parseNatSub n l su fa r) fa r;;
+
+let rec fst (x1, x2) = x1;;
+
+let rec divide_integer k l = fst (divmod_integer k l);;
+
+let rec divide_int
+  k l = Int_of_integer (divide_integer (integer_of_int k) (integer_of_int l));;
+
+let rec less_eq_int
+  k l = Big_int.le_big_int (integer_of_int k) (integer_of_int l);;
+
+let rec log256floor
+  x = (if less_eq_int x (Int_of_integer (Big_int.big_int_of_int 255))
+        then zero_int
+        else plus_int one_inta
+               (log256floor
+                 (divide_int x
+                   (Int_of_integer (Big_int.big_int_of_int 256)))));;
+
+let rec run_parse
+  p donea dfl s =
+    p s (fun x _ -> donea x) (fun _ -> dfl)
+      (fun sa _ _ -> run_parse p donea dfl sa);;
+
+let rec modulo_nat
+  m n = Nat (modulo_integer (integer_of_nat m) (integer_of_nat n));;
+
+let rec divide_nat
+  m n = Nat (divide_integer (integer_of_nat m) (integer_of_nat n));;
+
+let rec divmod_nat m n = (divide_nat m n, modulo_nat m n);;
+
+let rec nat_to_bytes
+  n = (let (a, mo) = divmod_nat n (nat_of_integer (Big_int.big_int_of_int 256))
+         in
+        (if equal_nat a zero_nat then [byteFromNat mo]
+          else byteFromNat mo :: nat_to_bytes (suc (minus_nat a one_nat))));;
+
+let rec output_address n = rev (nat_to_bytes n);;
+
+let rec intToBytes i = output_address (nat i);;
+
+let rec stree_append x0 uu = match x0, uu with STStr x, uu -> STStr x
+                       | STStrs xs, s -> STStrs (xs @ [s]);;
+
+let rec llll_parse
+  x0 uu uv = match x0, uu, uv with [], uu, uv -> None
+    | h :: t, token, parsed ->
+        (if ((h : char) = '(') then llll_parse t token (STStrs [] :: parsed)
+          else (if ((h : char) = ')')
+                 then (match parsed with [] -> None
+                        | [ph] ->
+                          (if not (null token)
+                            then Some (stree_append ph (STStr token))
+                            else Some ph)
+                        | ph :: ph2 :: pt ->
+                          (if not (null token)
+                            then llll_parse t []
+                                   (stree_append ph2
+                                      (stree_append ph (STStr token)) ::
+                                     pt)
+                            else llll_parse t [] (stree_append ph2 ph :: pt)))
+                 else (if isWs h
+                        then (if not (null token)
+                               then (match parsed with [] -> None
+                                      | ph :: pt ->
+llll_parse t [] (stree_append ph (STStr token) :: pt))
+                               else llll_parse t [] parsed)
+                        else llll_parse t (token @ [h]) parsed)));;
+
+let rec llll_parse0 s = llll_parse s [] [];;
+
+let rec run_parse_opt p f s = run_parse p f None s;;
+
+let rec run_parse_opta p s = run_parse_opt p (fun a -> Some a) s;;
+
+let rec llll_parse1
+  ft x1 = match ft, x1 with
+    ft, STStr s ->
+      (match run_parse_opta parseHex s
+        with None ->
+          (match run_parse_opta parseNat s
+            with None ->
+              (match lookupS ft s with None -> None
+                | Some f ->
+                  (match f [] with None -> None
+                    | Some l -> Some (l, (None, ft))))
+            | Some n -> Some (L4L_Nat n, (None, ft)))
+        | Some n -> Some (L4L_Nat n, (None, ft)))
+    | ft, STStrs (h :: t) ->
+        (match h
+          with STStr hs ->
+            (if equal_list equal_char hs ['d'; 'e'; 'f']
+              then (match t with [] -> None | [STStr _] -> None
+                     | [STStr h2; STStr listaa] ->
+                       (match llll_parse1_def h2 ft [] [STStr listaa]
+                         with None -> None | Some a -> Some a)
+                     | STStr _ :: STStr _ :: _ :: _ -> None
+                     | [STStr h2; STStrs l] ->
+                       (match llll_parse1_def h2 ft [] [STStrs l]
+                         with None -> None | Some a -> Some a)
+                     | [STStr h2; STStrs l; d] ->
+                       (match llll_parse1_def h2 ft [] (l @ [d])
+                         with None -> None | Some a -> Some a)
+                     | STStr _ :: STStrs _ :: _ :: _ :: _ -> None
+                     | STStrs _ :: _ -> None)
+              else (if equal_list equal_char hs
+                         ['r'; 'e'; 't'; 'u'; 'r'; 'n'; 'l'; 'l'; 'l']
+                     then (match t with [] -> None
+                            | [paysrc] ->
+                              (match llll_parse1 ft paysrc with None -> None
+                                | Some (ls, (None, fta)) ->
+                                  Some (L4Seq [], (Some ls, fta))
+                                | Some (_, (Some _, _)) -> None)
+                            | _ :: _ :: _ -> None)
+                     else (match lookupS ft hs with None -> None
+                            | Some f ->
+                              (match llll_parse1_args ft t with None -> None
+                                | Some (ls, (x, fta)) ->
+                                  (match f ls with None -> None
+                                    | Some l -> Some (l, (x, fta)))))))
+          | STStrs _ -> None)
+    | ft, STStrs [] -> None
+and llll_parse1_def
+  s ft vt x3 = match s, ft, vt, x3 with s, ft, vt, [] -> None
+    | name, ft, vt, [h] ->
+        (match name with [] -> None | [_] -> None
+          | hdchr :: aa :: lista ->
+            (if not ((hdchr : char) = apos) then None
+              else Some (L4Seq [],
+                          (None,
+                            (aa :: lista,
+                              (fun l ->
+                                (match mkConsts vt (rev l) with None -> None
+                                  | Some fta ->
+                                    (match llll_parse1 (fta @ ft) h
+                                      with None -> None
+                                      | Some (la, (_, _)) -> Some la)))) ::
+                              ft))))
+    | name, ft, vt, h :: v :: va ->
+        (match h with STStr vb -> llll_parse1_def name ft (vb :: vt) (v :: va)
+          | STStrs _ -> None)
+and llll_parse1_args
+  ft x1 = match ft, x1 with ft, [] -> None
+    | ft, [h] ->
+        (match llll_parse1 ft h with None -> None
+          | Some (l, (x, fta)) -> Some ([l], (x, fta)))
+    | ft, h :: v :: va ->
+        (match llll_parse1 ft h with None -> None
+          | Some (ha, (None, fta)) ->
+            (match llll_parse1_args fta (v :: va) with None -> None
+              | Some (t, (x, ftb)) -> Some (ha :: t, (x, ftb)))
+          | Some (ha, (Some pay, fta)) -> Some ([ha], (Some pay, fta)));;
+
+let rec mynth
+  x0 uu = match x0, uu with [], uu -> None
+    | h :: t, v ->
+        (if equal_nat v zero_nat then h
+          else mynth t (minus_nat (suc (minus_nat v one_nat)) one_nat));;
+
+let rec hexwrite1
+  c = (if equal_nat c zero_nat then '0'
+        else (if equal_nat c one_nat then '1'
+               else (if equal_nat c (nat_of_integer (Big_int.big_int_of_int 2))
+                      then '2'
+                      else (if equal_nat c
+                                 (nat_of_integer (Big_int.big_int_of_int 3))
+                             then '3'
+                             else (if equal_nat c
+(nat_of_integer (Big_int.big_int_of_int 4))
+                                    then '4'
+                                    else (if equal_nat c
+       (nat_of_integer (Big_int.big_int_of_int 5))
+   then '5'
+   else (if equal_nat c (nat_of_integer (Big_int.big_int_of_int 6)) then '6'
+          else (if equal_nat c (nat_of_integer (Big_int.big_int_of_int 7))
+                 then '7'
+                 else (if equal_nat c
+                            (nat_of_integer (Big_int.big_int_of_int 8))
+                        then '8'
+                        else (if equal_nat c
+                                   (nat_of_integer (Big_int.big_int_of_int 9))
+                               then '9'
+                               else (if equal_nat c
+  (nat_of_integer (Big_int.big_int_of_int 10))
+                                      then 'a'
+                                      else (if equal_nat c
+         (nat_of_integer (Big_int.big_int_of_int 11))
+     then 'b'
+     else (if equal_nat c (nat_of_integer (Big_int.big_int_of_int 12)) then 'c'
+            else (if equal_nat c (nat_of_integer (Big_int.big_int_of_int 13))
+                   then 'd'
+                   else (if equal_nat c
+                              (nat_of_integer (Big_int.big_int_of_int 14))
+                          then 'e'
+                          else (if equal_nat c
+                                     (nat_of_integer
+                                       (Big_int.big_int_of_int 15))
+                                 then 'f'
+                                 else failwith "undefined"))))))))))))))));;
+
+let rec hexwrite2
+  w = (let (d, m) =
+         divmod_nat (unat (len0_bit0 (len0_bit0 (len0_bit0 len0_num1))) w)
+           (nat_of_integer (Big_int.big_int_of_int 16))
+         in
+        (hexwrite1 d, hexwrite1 m));;
+
+let rec hexwrite
+  = function [] -> []
+    | h :: t -> (let (c1, c2) = hexwrite2 h in c1 :: c2 :: hexwrite t);;
+
+let rec nat_of_char
+  x = comp nat_of_integer (fun a -> Big_int.big_int_of_int (Char.code a)) x;;
+
+let rec truncate_string_sub
+  x0 n = match x0, n with
+    [], n ->
+      (if equal_nat n zero_nat then []
+        else byteFromNat zero_nat ::
+               truncate_string_sub [] (minus_nat n one_nat))
+    | h :: t, n ->
+        (if equal_nat n zero_nat then []
+          else byteFromNat (nat_of_char h) ::
+                 truncate_string_sub t (minus_nat n one_nat));;
+
+let rec truncate_string
+  s = truncate_string_sub s (nat_of_integer (Big_int.big_int_of_int 32));;
+
+let rec llll_compile
+  = function L4L_Str s -> L (Stack (PUSH_N (truncate_string s)))
+    | L4L_Nat i -> L (Stack (PUSH_N (intToBytes (int_of_nat i))))
+    | L4I0 i -> L i
+    | L4I1 (i, l) -> LSeq [llll_compile l; L i]
+    | L4I2 (i, l1, l2) -> LSeq [llll_compile l2; llll_compile l1; L i]
+    | L4Seq l -> LSeq (map llll_compile l)
+    | L4When (c, l) ->
+        LSeq [llll_compile c; L (Arith ISZERO); LJmpI zero_nat; llll_compile l;
+               LLab zero_nat]
+    | L4If (c, l1, l2) ->
+        LSeq [LSeq [llll_compile c; LJmpI zero_nat; llll_compile l2;
+                     LJmp one_nat; LLab zero_nat; llll_compile l1;
+                     LLab one_nat]]
+    | L4While (c, l) ->
+        LSeq [LSeq [LSeq [LLab zero_nat; llll_compile c; LJmpI one_nat;
+                           LJmp (nat_of_integer (Big_int.big_int_of_int 2));
+                           LLab one_nat; llll_compile l; LJmp zero_nat;
+                           LLab (nat_of_integer (Big_int.big_int_of_int 2))]]]
+    | L4Arith (LAPlus, ls) -> LSeq (map llll_compile (rev ls) @ [L (Arith ADD)])
+    | L4Arith (LAExp, ls) -> LSeq (map llll_compile (rev ls) @ [L (Arith EXP)])
+    | L4Arith (LADiv, ls) -> LSeq (map llll_compile (rev ls) @ [L (Arith DIV)])
+    | L4Comp (LCEq, l1, l2) ->
+        LSeq [llll_compile l2; llll_compile l1; L (Arith Inst_EQ)];;
+
+let rec mypeel
+  = function [] -> Some []
+    | None :: uu -> None
+    | Some h :: t ->
+        (match mypeel t with None -> None | Some ta -> Some (h :: ta));;
+
+let rec zero_word _A = word_of_int _A zero_int;;
+
+let base_interlude_size : nat = nat_of_integer (Big_int.big_int_of_int 9);;
+
+let rec makeInterlude
+  startbytes endbytes prelude payload =
+    prelude @
+      [Stack (PUSH_N (output_address (ilsz payload)))] @
+        [Dup (zero_word (len0_bit0 (len0_bit0 len0_num1)))] @
+          [Stack (PUSH_N
+                   (output_address
+                     (plus_nat
+                       (plus_nat (plus_nat (ilsz prelude) startbytes) endbytes)
+                       base_interlude_size)))] @
+            [Stack (PUSH_N (output_address zero_nat))] @
+              [Memory CODECOPY] @
+                [Stack (PUSH_N (output_address zero_nat))] @
+                  [Misc RETURN] @ payload;;
+
+let rec codegena
+  = function (uu, La (uv, i)) -> [i]
+    | (uw, LLaba (ux, uy)) -> [Pc JUMPDEST]
+    | (uz, LJmpa (a, va, s)) -> [Stack (PUSH_N (output_address a)); Pc JUMP]
+    | (vb, LJmpIa (a, vc, vd)) -> [Stack (PUSH_N (output_address a)); Pc JUMPI]
+    | (ve, LSeqa (vf, ls)) -> maps codegena ls;;
+
+let rec codegen ls = maps inst_code (codegena ls);;
+
+let rec ll3_bump
+  n x1 = match n, x1 with
+    n, ((xa, x), LSeqa (e, lsdec)) :: ls ->
+      ((plus_nat xa n, plus_nat x n), LSeqa (e, ll3_bump n lsdec)) ::
+        ll3_bump n ls
+    | n, ((xa, x), La (v, va)) :: ls ->
+        ((plus_nat xa n, plus_nat x n), La (v, va)) :: ll3_bump n ls
+    | n, ((xa, x), LLaba (v, va)) :: ls ->
+        ((plus_nat xa n, plus_nat x n), LLaba (v, va)) :: ll3_bump n ls
+    | n, ((xa, x), LJmpa (v, va, vb)) :: ls ->
+        ((plus_nat xa n, plus_nat x n), LJmpa (v, va, vb)) :: ll3_bump n ls
+    | n, ((xa, x), LJmpIa (v, va, vb)) :: ls ->
+        ((plus_nat xa n, plus_nat x n), LJmpIa (v, va, vb)) :: ll3_bump n ls
+    | n, [] -> [];;
+
+let rec ll3_init = function (x, La (e, i)) -> (x, La (e, i))
+                   | (x, LLaba (e, idx)) -> (x, LLaba (false, idx))
+                   | (x, LJmpa (e, idx, s)) -> (x, LJmpa (e, idx, s))
+                   | (x, LJmpIa (e, idx, s)) -> (x, LJmpIa (e, idx, s))
+                   | (x, LSeqa (e, ls)) -> (x, LSeqa ([], map ll3_init ls));;
+
+let rec ll4_init = function (x, La (e, i)) -> (x, La (e, i))
+                   | (x, LLaba (e, idx)) -> (x, LLaba (e, idx))
+                   | (x, LJmpa (e, idx, s)) -> (x, LJmpa (zero_nat, idx, s))
+                   | (x, LJmpIa (e, idx, s)) -> (x, LJmpIa (zero_nat, idx, s))
+                   | (x, LSeqa (e, ls)) -> (x, LSeqa (e, map ll4_init ls));;
+
+let rec ll_phase1
+  x0 i = match x0, i with
+    L inst, i ->
+      (((i, plus_nat i (nat (inst_size inst))), La ((), inst)),
+        plus_nat i (nat (inst_size inst)))
+    | LLab idx, i ->
+        (((i, plus_nat i one_nat), LLaba ((), idx)), plus_nat one_nat i)
+    | LJmp idx, i ->
+        (((i, plus_nat (nat_of_integer (Big_int.big_int_of_int 2)) i),
+           LJmpa ((), idx, zero_nat)),
+          plus_nat (nat_of_integer (Big_int.big_int_of_int 2)) i)
+    | LJmpI idx, i ->
+        (((i, plus_nat (nat_of_integer (Big_int.big_int_of_int 2)) i),
+           LJmpIa ((), idx, zero_nat)),
+          plus_nat (nat_of_integer (Big_int.big_int_of_int 2)) i)
+    | LSeq ls, i ->
+        (let (lsa, ia) = ll_phase1_seq ls i in (((i, ia), LSeqa ((), lsa)), ia))
+and ll_phase1_seq
+  x0 i = match x0, i with [], i -> ([], i)
+    | h :: t, i -> (let (ha, ia) = ll_phase1 h i in
+                    let a = ll_phase1_seq t ia in
+                    let (ta, aa) = a in
+                     (ha :: ta, aa));;
+
+let rec ll_pass1 l = fst (ll_phase1 l zero_nat);;
+
+let rec ll_get_label
+  vd ve = match vd, ve with [], ve -> None
+    | (vb, La (vf, vg)) :: va, [] -> None
+    | (vb, LJmpa (vf, vg, vh)) :: va, [] -> None
+    | (vb, LJmpIa (vf, vg, vh)) :: va, [] -> None
+    | (vb, LSeqa (vf, vg)) :: va, [] -> None
+    | vd, [] -> None
+    | (v, La (vd, ve)) :: ls, va :: vb ->
+        (if equal_nat va zero_nat then None
+          else ll_get_label ls
+                 (minus_nat (suc (minus_nat va one_nat)) one_nat :: vb))
+    | (v, LJmpa (vd, ve, vf)) :: ls, va :: vb ->
+        (if equal_nat va zero_nat then None
+          else ll_get_label ls
+                 (minus_nat (suc (minus_nat va one_nat)) one_nat :: vb))
+    | (v, LJmpIa (vd, ve, vf)) :: ls, va :: vb ->
+        (if equal_nat va zero_nat then None
+          else ll_get_label ls
+                 (minus_nat (suc (minus_nat va one_nat)) one_nat :: vb))
+    | (uy, LSeqa (uz, lsdec)) :: ls, va :: p ->
+        (if equal_nat va zero_nat then ll_get_label lsdec p
+          else ll_get_label ls
+                 (minus_nat (suc (minus_nat va one_nat)) one_nat :: p))
+    | ((x, uu), LLaba (uv, uw)) :: ux, [v] ->
+        (if equal_nat v zero_nat then Some x
+          else ll_get_label ux [minus_nat (suc (minus_nat v one_nat)) one_nat])
+    | (vb, LLaba (ve, vf)) :: ls, v :: va :: vc ->
+        (if equal_nat v zero_nat then None
+          else ll_get_label ls
+                 (minus_nat (suc (minus_nat v one_nat)) one_nat :: va :: vc));;
+
+let rec write_jump_targets
+  ns x1 = match ns, x1 with
+    ns, ((xa, x), LSeqa ([], lsdec)) ->
+      (match mypeel (map (write_jump_targets (None :: ns)) lsdec)
+        with None -> None | Some lsdeca -> Some ((xa, x), LSeqa ([], lsdeca)))
+    | ns, ((xa, x), LSeqa (v :: va, lsdec)) ->
+        (match ll_get_label lsdec (v :: va) with None -> None
+          | Some addr ->
+            (match mypeel (map (write_jump_targets (Some addr :: ns)) lsdec)
+              with None -> None
+              | Some lsdeca -> Some ((xa, x), LSeqa (v :: va, lsdeca))))
+    | ns, ((xa, x), LJmpa (uu, idx, sz)) ->
+        (match mynth ns idx with None -> None
+          | Some a -> Some ((xa, x), LJmpa (a, idx, sz)))
+    | ns, ((xa, x), LJmpIa (uv, idx, sz)) ->
+        (match mynth ns idx with None -> None
+          | Some a -> Some ((xa, x), LJmpIa (a, idx, sz)))
+    | uw, (v, La (vb, vc)) -> Some (v, La (vb, vc))
+    | uw, (v, LLaba (vb, vc)) -> Some (v, LLaba (vb, vc));;
+
+let rec encode_size n = plus_nat (nat (log256floor (int_of_nat n))) one_nat;;
+
+let rec ll3_resolve_jump
+  x0 oaddr n rel absol = match x0, oaddr, n, rel, absol with
+    (uu, LJmpa (e, idx, s)) :: ls, None, n, rel, absol ->
+      (if equal_nat (plus_nat idx one_nat) (size_list rel)
+        then JFail (n :: absol)
+        else ll3_resolve_jump ls None (plus_nat n one_nat) rel absol)
+    | (uv, LJmpa (e, idx, s)) :: ls, Some addr, n, rel, absol ->
+        (if equal_nat idx (size_list rel)
+          then (if less_nat s (encode_size addr) then JBump (n :: absol)
+                 else (if equal_nat s (encode_size addr)
+                        then ll3_resolve_jump ls (Some addr)
+                               (plus_nat n one_nat) rel absol
+                        else JFail (n :: absol)))
+          else ll3_resolve_jump ls (Some addr) (plus_nat n one_nat) rel absol)
+    | (uw, LJmpIa (e, idx, s)) :: ls, None, n, rel, absol ->
+        (if equal_nat (plus_nat idx one_nat) (size_list rel)
+          then JFail (n :: absol)
+          else ll3_resolve_jump ls None (plus_nat n one_nat) rel absol)
+    | (ux, LJmpIa (e, idx, s)) :: ls, Some addr, n, rel, absol ->
+        (if equal_nat idx (size_list rel)
+          then (if less_nat s (encode_size addr) then JBump (n :: absol)
+                 else (if equal_nat s (encode_size addr)
+                        then ll3_resolve_jump ls (Some addr)
+                               (plus_nat n one_nat) rel absol
+                        else JFail (n :: absol)))
+          else ll3_resolve_jump ls (Some addr) (plus_nat n one_nat) rel absol)
+    | (uy, LSeqa ([], lsdec)) :: ls, oaddr, n, rel, absol ->
+        (match ll3_resolve_jump lsdec oaddr zero_nat (n :: rel) (n :: absol)
+          with JSuccess ->
+            (match ll3_resolve_jump lsdec None zero_nat [] (n :: absol)
+              with JSuccess ->
+                ll3_resolve_jump ls oaddr (plus_nat n one_nat) rel absol
+              | JFail a -> JFail a | JBump a -> JBump a)
+          | JFail a -> JFail a | JBump a -> JBump a)
+    | (uz, LSeqa (v :: va, lsdec)) :: ls, oaddr, n, rel, absol ->
+        (match ll3_resolve_jump lsdec oaddr zero_nat (n :: rel) (n :: absol)
+          with JSuccess ->
+            (match ll_get_label lsdec (v :: va) with None -> JFail absol
+              | Some newaddr ->
+                (match
+                  ll3_resolve_jump lsdec (Some newaddr) zero_nat [] (n :: absol)
+                  with JSuccess ->
+                    ll3_resolve_jump ls oaddr (plus_nat n one_nat) rel absol
+                  | JFail a -> JFail a | JBump a -> JBump a))
+          | JFail a -> JFail a | JBump a -> JBump a)
+    | (v, La (vb, vc)) :: ls, oaddr, n, rel, absol ->
+        ll3_resolve_jump ls oaddr (plus_nat n one_nat) rel absol
+    | (v, LLaba (vb, vc)) :: ls, oaddr, n, rel, absol ->
+        ll3_resolve_jump ls oaddr (plus_nat n one_nat) rel absol
+    | [], va, vb, vc, vd -> JSuccess;;
+
+let rec ll3_resolve_jump_wrap
+  = function
+    (x, LSeqa (e, lsdec)) ->
+      (match e with [] -> ll3_resolve_jump lsdec None zero_nat [] []
+        | a :: lista ->
+          (match ll_get_label lsdec (a :: lista) with None -> JFail []
+            | Some aa -> ll3_resolve_jump lsdec (Some aa) zero_nat [] []))
+    | (v, La (vb, vc)) -> JFail []
+    | (v, LLaba (vb, vc)) -> JFail []
+    | (v, LJmpa (vb, vc, vd)) -> JFail []
+    | (v, LJmpIa (vb, vc, vd)) -> JFail [];;
+
+let rec ll3_inc_jump
+  x0 n c = match x0, n, c with
+    ((xa, x), LJmpa (e, idx, s)) :: ls, n, [c] ->
+      (if equal_nat n c
+        then (((xa, plus_nat x one_nat), LJmpa (e, idx, plus_nat s one_nat)) ::
+                ll3_bump one_nat ls,
+               true)
+        else (let (lsa, a) = ll3_inc_jump ls (plus_nat n one_nat) [c] in
+               (((xa, x), LJmpa (e, idx, s)) :: lsa, a)))
+    | ((xa, x), LJmpIa (e, idx, s)) :: ls, n, [c] ->
+        (if equal_nat n c
+          then (((xa, plus_nat x one_nat),
+                  LJmpIa (e, idx, plus_nat s one_nat)) ::
+                  ll3_bump one_nat ls,
+                 true)
+          else (let (lsa, a) = ll3_inc_jump ls (plus_nat n one_nat) [c] in
+                 (((xa, x), LJmpIa (e, idx, s)) :: lsa, a)))
+    | ((xa, x), LSeqa (e, lsdec)) :: ls, n, c :: cs ->
+        (if equal_nat n c
+          then (match ll3_inc_jump lsdec zero_nat cs
+                 with (lsdeca, true) ->
+                   (((xa, plus_nat x one_nat), LSeqa (e, lsdeca)) ::
+                      ll3_bump one_nat ls,
+                     true)
+                 | (lsdeca, false) ->
+                   (let (lsa, a) = ll3_inc_jump ls n (c :: cs) in
+                     (((xa, x), LSeqa (e, lsdeca)) :: lsa, a)))
+          else (let (lsa, a) = ll3_inc_jump ls (plus_nat n one_nat) (c :: cs) in
+                 (((xa, x), LSeqa (e, lsdec)) :: lsa, a)))
+    | (v, La (vb, vc)) :: ls, n, c ->
+        (let (lsa, a) = ll3_inc_jump ls (plus_nat n one_nat) c in
+          ((v, La (vb, vc)) :: lsa, a))
+    | (v, LLaba (vb, vc)) :: ls, n, c ->
+        (let (lsa, a) = ll3_inc_jump ls (plus_nat n one_nat) c in
+          ((v, LLaba (vb, vc)) :: lsa, a))
+    | (v, LJmpIa (vb, vc, vd)) :: ls, n, [] ->
+        (let (lsa, a) = ll3_inc_jump ls (plus_nat n one_nat) [] in
+          ((v, LJmpIa (vb, vc, vd)) :: lsa, a))
+    | (v, LJmpIa (vb, vc, vd)) :: ls, n, va :: vf :: vg ->
+        (let (lsa, a) = ll3_inc_jump ls (plus_nat n one_nat) (va :: vf :: vg) in
+          ((v, LJmpIa (vb, vc, vd)) :: lsa, a))
+    | (v, LSeqa (vb, vc)) :: ls, n, [] ->
+        (let (lsa, a) = ll3_inc_jump ls (plus_nat n one_nat) [] in
+          ((v, LSeqa (vb, vc)) :: lsa, a))
+    | h :: ls, n, [] ->
+        (let (lsa, a) = ll3_inc_jump ls (plus_nat n one_nat) [] in
+          (h :: lsa, a))
+    | (va, LJmpa (ve, vf, vg)) :: ls, n, v :: vb :: vc ->
+        (let (lsa, a) = ll3_inc_jump ls (plus_nat n one_nat) (v :: vb :: vc) in
+          ((va, LJmpa (ve, vf, vg)) :: lsa, a))
+    | [], uu, uv -> ([], false);;
+
+let rec ll3_inc_jump_wrap
+  x0 c = match x0, c with
+    ((xa, x), LSeqa (e, lsdec)), c ->
+      (match ll3_inc_jump lsdec zero_nat c
+        with (lsdeca, true) -> ((xa, plus_nat x one_nat), LSeqa (e, lsdeca))
+        | (_, false) -> ((xa, x), LSeqa (e, lsdec)))
+    | (v, La (vb, vc)), uu -> (v, La (vb, vc))
+    | (v, LLaba (vb, vc)), uu -> (v, LLaba (vb, vc))
+    | (v, LJmpa (vb, vc, vd)), uu -> (v, LJmpa (vb, vc, vd))
+    | (v, LJmpIa (vb, vc, vd)), uu -> (v, LJmpIa (vb, vc, vd));;
+
+let rec process_jumps_loop
+  v uu =
+    (if equal_nat v zero_nat then None
+      else (match ll3_resolve_jump_wrap uu with JSuccess -> Some uu
+             | JFail _ -> None
+             | JBump c ->
+               process_jumps_loop
+                 (minus_nat (suc (minus_nat v one_nat)) one_nat)
+                 (ll3_inc_jump_wrap uu (rev c))));;
+
+let rec equal_bool p pa = match p, pa with p, true -> p
+                     | p, false -> not p
+                     | true, p -> p
+                     | false, p -> not p;;
+
+let rec ll3_consume_label
+  p n x2 = match p, n, x2 with p, n, [] -> Some ([], [])
+    | p, n, (x, LLaba (b, idx)) :: ls ->
+        (if equal_nat idx (size_list p)
+          then (if equal_bool b false
+                 then Some ((x, LLaba (true, idx)) :: ls, n :: p) else None)
+          else (match ll3_consume_label p (plus_nat n one_nat) ls
+                 with None -> None
+                 | Some (lsa, pa) -> Some ((x, LLaba (b, idx)) :: lsa, pa)))
+    | p, n, (x, LSeqa (e, lsdec)) :: ls ->
+        (match ll3_consume_label (n :: p) zero_nat lsdec with None -> None
+          | Some (lsdeca, []) ->
+            (match ll3_consume_label p (plus_nat n one_nat) ls with None -> None
+              | Some (lsa, pa) -> Some ((x, LSeqa (e, lsdeca)) :: lsa, pa))
+          | Some (lsdeca, aa :: lista) ->
+            Some ((x, LSeqa (e, lsdeca)) :: ls, aa :: lista))
+    | p, n, (v, La (vb, vc)) :: ls ->
+        (match ll3_consume_label p (plus_nat n one_nat) ls with None -> None
+          | Some (lsa, pa) -> Some ((v, La (vb, vc)) :: lsa, pa))
+    | p, n, (v, LJmpa (vb, vc, vd)) :: ls ->
+        (match ll3_consume_label p (plus_nat n one_nat) ls with None -> None
+          | Some (lsa, pa) -> Some ((v, LJmpa (vb, vc, vd)) :: lsa, pa))
+    | p, n, (v, LJmpIa (vb, vc, vd)) :: ls ->
+        (match ll3_consume_label p (plus_nat n one_nat) ls with None -> None
+          | Some (lsa, pa) -> Some ((v, LJmpIa (vb, vc, vd)) :: lsa, pa));;
+
+let rec ll3_assign_label
+  = function
+    (x, LSeqa (e, ls)) ->
+      (match ll3_consume_label [] zero_nat ls with None -> None
+        | Some (lsa, p) ->
+          (match ll3_assign_label_list lsa with None -> None
+            | Some lsb -> Some (x, LSeqa (rev p, lsb))))
+    | (x, LLaba (false, idx)) -> None
+    | (v, La (vb, vc)) -> Some (v, La (vb, vc))
+    | (v, LLaba (true, vc)) -> Some (v, LLaba (true, vc))
+    | (v, LJmpa (vb, vc, vd)) -> Some (v, LJmpa (vb, vc, vd))
+    | (v, LJmpIa (vb, vc, vd)) -> Some (v, LJmpIa (vb, vc, vd))
+and ll3_assign_label_list
+  = function [] -> Some []
+    | h :: t ->
+        (match ll3_assign_label h with None -> None
+          | Some ha ->
+            (match ll3_assign_label_list t with None -> None
+              | Some ta -> Some (ha :: ta)));;
+
+let rec pipelinea
+  l n = (match ll3_assign_label (ll3_init (ll_pass1 l)) with None -> None
+          | Some la ->
+            (match process_jumps_loop n la with None -> None
+              | Some lb ->
+                (match write_jump_targets [] (ll4_init lb) with None -> None
+                  | Some a -> Some a)));;
+
+let rec pipeline
+  l n = (match pipelinea l n with None -> None | Some la -> Some (codegen la));;
+
+let rec get_process_jumps_fuela
+  = function
+    (uu, LJmpa (uv, uw, s)) ->
+      minus_nat (nat_of_integer (Big_int.big_int_of_int 32)) s
+    | (ux, LJmpIa (uy, uz, s)) ->
+        minus_nat (nat_of_integer (Big_int.big_int_of_int 32)) s
+    | (va, LSeqa (vb, ls)) ->
+        foldl (fun a x -> plus_nat a (get_process_jumps_fuela x)) zero_nat ls
+    | (v, La (vb, vd)) -> zero_nat
+    | (v, LLaba (vb, vd)) -> zero_nat;;
+
+let rec get_process_jumps_fuel
+  l = plus_nat one_nat (get_process_jumps_fuela l);;
+
+let rec llll_combine_payload_sub
+  fuel presz paysz startbytes endbytes =
+    (if equal_nat fuel zero_nat then None
+      else (if equal_nat (encode_size paysz) endbytes
+             then (if equal_nat
+                        (encode_size
+                          (plus_nat
+                            (plus_nat (plus_nat presz startbytes) endbytes)
+                            base_interlude_size))
+                        startbytes
+                    then Some (startbytes, endbytes)
+                    else llll_combine_payload_sub (minus_nat fuel one_nat) presz
+                           paysz (plus_nat startbytes one_nat) endbytes)
+             else llll_combine_payload_sub (minus_nat fuel one_nat) presz paysz
+                    startbytes (plus_nat endbytes one_nat)));;
+
+let combine_payload_fuel : nat
+  = plus_nat (nat_of_integer (Big_int.big_int_of_int 32))
+      (nat_of_integer (Big_int.big_int_of_int 32));;
+
+let default_llll_funs : (char list * (llll list -> llll option)) list
+  = [(['s'; 'e'; 'q'], (fun l -> Some (L4Seq l)));
+      (['i'; 'f'],
+        (fun a ->
+          (match a with [] -> None | [_] -> None | [_; _] -> None
+            | [c; br1; br2] -> Some (L4If (c, br1, br2))
+            | _ :: _ :: _ :: _ :: _ -> None)));
+      (['w'; 'h'; 'e'; 'n'],
+        (fun a ->
+          (match a with [] -> None | [_] -> None
+            | [c; br] -> Some (L4When (c, br)) | _ :: _ :: _ :: _ -> None)));
+      (['+'], (fun l -> Some (L4Arith (LAPlus, l))));
+      (['-'], (fun l -> Some (L4Arith (LAMinus, l))));
+      (['*'], (fun l -> Some (L4Arith (LATimes, l))));
+      (['d'; 'i'; 'v'], (fun l -> Some (L4Arith (LADiv, l))));
+      (['e'; 'x'; 'p'], (fun l -> Some (L4Arith (LAExp, l))));
+      (['/'], (fun l -> Some (L4Arith (LADiv, l))));
+      (['%'], (fun l -> Some (L4Arith (LAMod, l))));
+      (['&'], (fun l -> Some (L4Arith (LAAnd, l))));
+      (['|'], (fun l -> Some (L4Arith (LAOr, l))));
+      (['^'], (fun l -> Some (L4Arith (LAXor, l))));
+      (['~'], (fun l -> Some (L4Arith (LANot, l))));
+      (['&'; '&'], (fun l -> Some (L4Logic (LLAnd, l))));
+      (['|'; '|'], (fun l -> Some (L4Logic (LLOr, l))));
+      (['!'], (fun l -> Some (L4Logic (LLNot, l))));
+      (['='],
+        (fun a ->
+          (match a with [] -> None | [_] -> None
+            | [lhs; rhs] -> Some (L4Comp (LCEq, lhs, rhs))
+            | _ :: _ :: _ :: _ -> None)));
+      (['m'; 's'; 't'; 'o'; 'r'; 'e'],
+        (fun a ->
+          (match a with [] -> None | [_] -> None
+            | [loc; sz] -> Some (L4I2 (Memory MSTORE, loc, sz))
+            | _ :: _ :: _ :: _ -> None)));
+      (['r'; 'e'; 't'; 'u'; 'r'; 'n'],
+        (fun a ->
+          (match a with [] -> None | [_] -> None
+            | [loc; sz] -> Some (L4I2 (Misc RETURN, loc, sz))
+            | _ :: _ :: _ :: _ -> None)));
+      (['c'; 'a'; 'l'; 'l'; 'd'; 'a'; 't'; 'a'; 'l'; 'o'; 'a'; 'd'],
+        (fun a ->
+          (match a with [] -> None
+            | [loc] -> Some (L4I1 (Stack CALLDATALOAD, loc))
+            | _ :: _ :: _ -> None)))];;
+
+let rec llll_parse1_default
+  st = (match llll_parse1 default_llll_funs st with None -> None
+         | Some (l, (x, _)) -> Some (l, x));;
+
+let rec llll_parse_complete
+  s = (match llll_parse0 s with None -> None
+        | Some a -> llll_parse1_default a);;
+
+let rec pipelineb
+  l n = (match pipelinea l n with None -> None
+          | Some la -> Some (codegena la));;
+
+let rec fourL_compiler_string
+  s = (match llll_parse_complete s with None -> None
+        | Some (l4pre, None) ->
+          (match
+            pipeline (llll_compile l4pre)
+              (get_process_jumps_fuel (ll_pass1 (llll_compile l4pre)))
+            with None -> None | Some wl -> Some (hexwrite wl))
+        | Some (l4pre, Some l4pay) ->
+          (match
+            pipelineb (llll_compile l4pre)
+              (get_process_jumps_fuel (ll_pass1 (llll_compile l4pre)))
+            with None -> None
+            | Some il_pre ->
+              (match
+                pipelineb (llll_compile l4pay)
+                  (get_process_jumps_fuel (ll_pass1 (llll_compile l4pay)))
+                with None -> None
+                | Some il_pay ->
+                  (match
+                    llll_combine_payload_sub combine_payload_fuel (ilsz il_pre)
+                      (ilsz il_pay) zero_nat zero_nat
+                    with None -> None
+                    | Some (startbytes, endbytes) ->
+                      Some (hexwrite
+                             (il2wl
+                               (makeInterlude startbytes endbytes il_pre
+                                 il_pay)))))));;
+
+let rec compiler
+  l = (match
+        fourL_compiler_string
+          (let s = l in let rec exp i l = if i < 0 then l else exp (i - 1) (String.get s i :: l) in exp (String.length s - 1) [])
+        with None -> None
+        | Some s ->
+          Some (let l = s in let res = String.create (List.length l) in let rec imp i = function | [] -> res | c :: l -> String.set res i c; imp (i + 1) l in imp 0 l));;
+
+end;; (*struct FourL*)
