elle/build_FourL.sh
@@ -1,3 +1,0 @@
-#!/bin/bash
-# needs to be run from generated/ directory
-# ocamlc -o llllc unix.cma nums.cma FourL.ml ../FourLShim.mli
